template-coq/theories/EnvironmentTyping.v
@@ -167,6 +167,63 @@ Module EnvTyping (T : Term) (E : EnvironmentSig T).
   Arguments localenv_cons_def {_ _ _ _ _} _ _.
   Arguments localenv_cons_abs {_ _ _ _} _ _.
 
+  Section All2_local_env.
+
+  Definition on_decl (P : context -> context -> term -> term -> Type)
+             (Γ Γ' : context) (b : option (term * term)) (t t' : term) :=
+    match b with
+    | Some (b, b') => (P Γ Γ' b b' * P Γ Γ' t t')%type
+    | None => P Γ Γ' t t'
+    end.
+
+  Section All_local_2.
+    Context (P : forall (Γ Γ' : context), option (term * term) -> term -> term -> Type).
+
+    Inductive All2_local_env : context -> context -> Type :=
+    | localenv2_nil : All2_local_env [] []
+    | localenv2_cons_abs Γ Γ' na na' t t' :
+        All2_local_env Γ Γ' ->
+        P Γ Γ' None t t' ->
+        All2_local_env (Γ ,, vass na t) (Γ' ,, vass na' t')
+    | localenv2_cons_def Γ Γ' na na' b b' t t' :
+        All2_local_env Γ Γ' ->
+        P Γ Γ' (Some (b, b')) t t' ->
+        All2_local_env (Γ ,, vdef na b t) (Γ' ,, vdef na' b' t').
+  End All_local_2.
+
+  Definition on_decl_over (P : context -> context -> term -> term -> Type) Γ Γ' :=
+    fun Δ Δ' => P (Γ ,,, Δ) (Γ' ,,, Δ').
+
+  Definition All2_local_env_over P Γ Γ' := All2_local_env (on_decl (on_decl_over P Γ Γ')).
+
+  Lemma All2_local_env_length {P l l'} : @All2_local_env P l l' -> #|l| = #|l'|.
+  Proof. induction 1; simpl; auto. Qed.
+
+
+  Lemma All2_local_env_impl {P Q : context -> context -> term -> term -> Type} {par par'} :
+    All2_local_env (on_decl P) par par' ->
+    (forall par par' x y, P par par' x y -> Q par par' x y) ->
+    All2_local_env (on_decl Q) par par'.
+  Proof.
+    intros H aux.
+    induction H; constructor. auto. red in p. apply aux, p.
+    apply IHAll2_local_env. red. split.
+    apply aux. apply p. apply aux. apply p.
+  Defined.
+
+  Lemma All2_local_env_app_inv :
+    forall P (Γ Γ' Γl Γr : context),
+      All2_local_env (on_decl P) Γ Γl ->
+      All2_local_env (on_decl (on_decl_over P Γ Γl)) Γ' Γr ->
+      All2_local_env (on_decl P) (Γ ,,, Γ') (Γl ,,, Γr).
+  Proof.
+    induction 2; auto.
+    - simpl. constructor; auto.
+    - simpl. constructor; auto.
+  Qed.
+
+  End All2_local_env.
+
   (** Well-formedness of local environments embeds a sorting for each variable *)
 
   Definition lift_typing (P : global_env_ext -> context -> term -> term -> Type) :
@@ -224,6 +281,9 @@ Module Type Typing (T : Term) (E : EnvironmentSig T) (ET : EnvTypingSig T E).
 
   Parameter (ind_guard : mutual_inductive_body -> bool).
 
+  Parameter (conv : forall `{checker_flags}, global_env_ext -> context -> term -> term -> Type).
+  Parameter (cumul : forall `{checker_flags}, global_env_ext -> context -> term -> term -> Type).
+
   Parameter (typing : forall `{checker_flags}, global_env_ext -> context -> term -> term -> Type).
 
   Notation " Σ ;;; Γ |- t : T " :=
@@ -232,6 +292,8 @@ Module Type Typing (T : Term) (E : EnvironmentSig T) (ET : EnvTypingSig T E).
   Parameter Inline smash_context : context -> context -> context.
   Parameter Inline lift_context : nat -> nat -> context -> context.
   Parameter Inline subst_telescope : list term -> nat -> context -> context.
+  Parameter Inline subst_instance_context : Instance.t -> context -> context.
+  Parameter Inline subst_instance_constr : Instance.t -> term  -> term.
   Parameter Inline lift : nat -> nat -> term -> term.
   Parameter Inline subst : list term -> nat -> term -> term.
   Parameter Inline inds : kername -> Instance.t -> list one_inductive_body -> list term.
@@ -396,6 +458,72 @@ Module DeclarationTyping (T : Term) (E : EnvironmentSig T)
       positive_cstr mdecl i (vass na ty :: ctx) t ->
       positive_cstr mdecl i ctx (tProd na ty t).
 
+    Definition lift_level n l :=
+      match l with 
+      | Level.lProp | Level.lSet | Level.Level _ => l
+      | Level.Var k => Level.Var (n + k)
+      end.
+
+    Definition lift_constraint n (c : Level.t * ConstraintType.t * Level.t) :=
+      let '((l, r), l') := c in
+      ((lift_level n l, r), lift_level n l').
+
+    Definition lift_constraints n cstrs :=
+      ConstraintSet.fold (fun elt acc => ConstraintSet.add (lift_constraint n elt) acc)
+        cstrs ConstraintSet.empty.
+
+    Definition level_var_instance n (inst : list name) :=
+      mapi_rec (fun i _ => Level.Var i) inst n.
+
+    Fixpoint add_variance (v : list Variance.t) (u u' : Instance.t) cstrs :=
+      match v, u, u' with
+      | _, [], [] => cstrs
+      | v :: vs, u :: us, u' :: us' => 
+        match v with
+        | Variance.Irrelevant => add_variance vs us us' cstrs
+        | Variance.Covariant => add_variance vs us us' (ConstraintSet.add (u, ConstraintType.Le, u') cstrs)
+        | Variance.Invariant => add_variance vs us us' (ConstraintSet.add (u, ConstraintType.Eq, u') cstrs)
+        end
+      | _, _, _ => (* Impossible *) cstrs
+      end.
+
+    (** This constructs a duplication of the polymorphic universe context of the inductive,  
+      where the two instances are additionally related according to the variance information.
+    *)
+
+    Definition variance_universes univs v :=
+      match univs with
+      | Monomorphic_ctx ctx => (univs, [], []) (* Dummy value: impossible case *)
+      | Polymorphic_ctx auctx =>
+        let (inst, cstrs) := auctx in
+        let u := level_var_instance #|inst| inst in
+        let u' := level_var_instance 0 inst in
+        let cstrs := ConstraintSet.union cstrs (lift_constraints #|inst| cstrs) in
+        let cstra := add_variance v u u' cstrs in
+        let auctx' := (inst ++ inst, cstrs) in
+        (Polymorphic_ctx auctx', u, u')
+      end.
+
+    (** A constructor type respects the given variance [v] if each constructor 
+        argument respects it and each index (in the conclusion) does as well.
+        We formalize this by asking for a cumulativity relation between the contexts
+        of arguments and conversion of the lists of indices instanciated with [u] and 
+        [u'] where [u `v` u']. *)
+
+    Definition ind_arities mdecl := arities_context (ind_bodies mdecl).
+
+    Definition respects_variance Σ mdecl v cs :=
+      let univs := ind_universes mdecl in
+      let '(univs, u, u') := variance_universes univs v in
+      All2_local_env 
+        (on_decl (fun Γ Γ' t t' => cumul (Σ, univs) (ind_arities mdecl ,,, ind_params mdecl ,,, Γ) t t'))
+        (subst_instance_context u (cshape_args cs))
+        (subst_instance_context u' (cshape_args cs)) *
+      All2 
+        (conv (Σ, univs) (ind_arities mdecl ,,, ind_params mdecl ,,, cshape_args cs))
+        (map (subst_instance_constr u) (cshape_indices cs))
+        (map (subst_instance_constr u') (cshape_indices cs)).
+
     Record on_constructor Σ mdecl i idecl ind_indices cdecl (cshape : constructor_shape) := {
       (* cdecl.1 fresh ?? *)
       cstr_args_length : context_assumptions (cshape_args cshape) = cdecl_args cdecl;
@@ -427,8 +555,12 @@ Module DeclarationTyping (T : Term) (E : EnvironmentSig T)
                       (List.rev (lift_context #|cshape.(cshape_args)| 0 ind_indices));
 
       on_ctype_positive : (* The constructor type is positive *)
-        positive_cstr mdecl i [] (cdecl_type cdecl)
+        positive_cstr mdecl i [] (cdecl_type cdecl);
 
+      on_ctype_variance : (* The constructor type respect the variance annotation 
+        on polymorphic universes, if any. *)
+        forall v, ind_variance mdecl = Some v -> 
+        respects_variance Σ mdecl v cshape
     }.
 
     Arguments on_ctype {Σ mdecl i idecl ind_indices cdecl cshape}.
@@ -651,11 +783,13 @@ Module DeclarationTyping (T : Term) (E : EnvironmentSig T)
 
   End GlobalMaps.
 
-  Arguments cstr_args_length {P Σ mdecl i idecl ind_indices cdecl cshape}.
-  Arguments cstr_eq {P Σ mdecl i idecl ind_indices cdecl cshape}.
-  Arguments on_ctype {P Σ mdecl i idecl ind_indices cdecl cshape}.
-  Arguments on_cargs {P Σ mdecl i idecl ind_indices cdecl cshape}.
-  Arguments on_cindices {P Σ mdecl i idecl ind_indices cdecl cshape}.
+  Arguments cstr_args_length {_ P Σ mdecl i idecl ind_indices cdecl cshape}.
+  Arguments cstr_eq {_ P Σ mdecl i idecl ind_indices cdecl cshape}.
+  Arguments on_ctype {_ P Σ mdecl i idecl ind_indices cdecl cshape}.
+  Arguments on_cargs {_ P Σ mdecl i idecl ind_indices cdecl cshape}.
+  Arguments on_cindices {_ P Σ mdecl i idecl ind_indices cdecl cshape}.
+  Arguments on_ctype_positive {_ P Σ mdecl i idecl ind_indices cdecl cshape}.
+  Arguments on_ctype_variance {_ P Σ mdecl i idecl ind_indices cdecl cshape}.
 
   Arguments ind_indices {_ P Σ mind mdecl i idecl}.
   Arguments ind_sort {_ P Σ mind mdecl i idecl}.
